Do 64 tests at once

SortingNetworkSearch/Basic.lean
@@ -29,8 +29,11 @@ theorem ByteArray.size_uset {xs : ByteArray} {v : UInt8} {i : USize} (h : i.toNa
 instance : Repr ByteArray where
   reprPrec b n := reprPrec b.toList.toArray n
 
-structure Network (size : UInt8) where
-  toArray : Array ByteArray
+abbrev Layer := Array USize
+abbrev Swap := USize × USize
+
+structure Network (size : USize) where
+  toArray : Array Layer
   deriving Repr, DecidableEq, Hashable
 
 def Network.instInhabited : Network size :=
@@ -40,7 +43,7 @@ def Network.instInhabited : Network size :=
 instance : Inhabited (Network size) where
   default := Network.instInhabited
 
-def Layer.toSwaps (layer : ByteArray) : Array (UInt8 × UInt8) :=
+def Layer.toSwaps (layer : Array USize) : Array Swap :=
   Prod.fst <| layer.foldl
     (init := (
       Array.emptyWithCapacity (layer.size / 2),
@@ -66,21 +69,21 @@ def ByteArray.range (n : UInt8) : ByteArray := Id.run do
     i := i + 1
   result
 
-def Swaps.toLayer (size : UInt8) (swaps : Array (UInt8 × UInt8)) : ByteArray :=
+def Swaps.toLayer (size : USize) (swaps : Array Swap) : Layer :=
   swaps.foldl
-    (init := .range size)
+    (init := Array.range size.toNat |>.map (·.toUSize))
     fun acc (a, b) =>
       let acc := acc.set! a.toNat b
       let acc := acc.set! b.toNat a
       acc
 
-def Network.toSwaps (n : Network size) : Array (UInt8 × UInt8) :=
+def Network.toSwaps (n : Network size) : Array Swap :=
   n.toArray.flatMap (Layer.toSwaps ·)
 
-def Network.fromLayerSwaps (layers : Array (Array (UInt8 × UInt8))) : Network size :=
+def Network.fromLayerSwaps (layers : Array (Array Swap)) : Network size :=
   Network.mk <|
     layers.map fun swaps =>
-      swaps.foldl (init := .range size)
+      swaps.foldl (init := Array.range size.toNat |>.map (·.toUSize))
         fun acc (a, b) =>
           let acc := acc.set! a.toNat b
           let acc := acc.set! b.toNat a
@@ -104,24 +107,58 @@ def binaryCompareAndSwap
   let val := val ||| aBit's ||| bBit's
   val
 
+@[grind →]
+theorem array_index_lt_size_ofNat_of_lt_usize
+    (vals : Array UInt64)
+    (a : USize)
+    (h : a < vals.usize)
+    : a < USize.ofNat vals.size := by
+  exact h
+
+attribute [grind =] USize.lt_ofNat_iff
+
+@[grind]
+structure binaryParallelCompareAndSwap.h (vals : Array UInt64) (a b : USize) where
+  size_vals_lt : vals.size < USize.size := by grind
+  a_lt_vals_usize : a < vals.usize
+  b_lt_vals_usize : b < vals.usize
+
+def binaryParallelCompareAndSwap
+    (a b : USize)
+    (vals : Subtype (binaryParallelCompareAndSwap.h · a b) )
+    : Array UInt64 :=
+  have : a.toNat < vals.val.size := by grind
+  have : b.toNat < vals.val.size := by grind
+  let tmp := vals.val[a]
+  let vals := vals.val.uset a (tmp &&& vals.val[b]) (by grind)
+  let vals := vals.uset b (tmp ||| vals[b]'(by grind)) (by grind)
+  vals
+
+@[grind =]
+theorem binaryParallelCompareAndSwap_size_eq
+    (a b : USize)
+    (vals : Subtype (binaryParallelCompareAndSwap.h · a b))
+    : (binaryParallelCompareAndSwap a b vals).size = vals.val.size := by
+  simp [binaryParallelCompareAndSwap]
+
 instance instMembershipByteArray : Membership UInt8 ByteArray where
   mem as a := a ∈ as.data
 
 @[grind]
-structure CompiledNetwork where
-  as : ByteArray
-  bs : ByteArray
+structure CompiledNetwork (size : USize) where
+  as : Array USize
+  bs : Array USize
   size_eq : as.size = bs.size := by grind
   size_lt_USize_size : as.size < USize.size := by grind
-  as_all_lt_64 : ∀ a ∈ as, a < 64 := by grind
-  bs_all_lt_64 : ∀ b ∈ bs, b < 64 := by grind
+  as_sizes : ∀ a ∈ as, a < size := by grind
+  bs_sizes : ∀ b ∈ bs, b < size := by grind
 
 attribute [grind →] ByteArray.size
 attribute [grind =] ByteArray.empty ByteArray.emptyWithCapacity
 attribute [grind] USize.size_pos
 
 theorem idk3
-    : ∀ a ∈ ByteArray.empty, a < 64 := by
+    : ∀ a ∈ ByteArray.empty, a < size := by
   unfold instMembershipByteArray
   grind
 
@@ -139,111 +176,307 @@ theorem ByteArray.size_empty_lt_Usize_size : empty.size < USize.size := by
 
 grind_pattern ByteArray.size_empty_lt_Usize_size => ByteArray.empty.size, USize.size
 
-instance : Inhabited CompiledNetwork where
-  default :=
-    have h_as : ∀ a ∈ ByteArray.empty, a < 64 := idk3
-    have h_bs : ∀ b ∈ ByteArray.empty, b < 64 := idk3
-    CompiledNetwork.mk .empty .empty
+instance { size : USize } : Inhabited (CompiledNetwork size) where
+  default := by
+    have h_as : ∀ a ∈ #[], a < size := by grind
+    have h_bs : ∀ b ∈ #[], b < size := by grind
+    refine CompiledNetwork.mk #[] #[] ?_ ?_ ?_ ?_
+    . grind
+    . rw [Array.size_empty]
+      exact USize.size_pos
+    . grind
+    . grind
 
 theorem idk1
-    (xs : Array (UInt8 × UInt8))
-    (h : as = ByteArray.mk xs.unzip.fst)
-    (h : as.data.all (· < 64))
-    : ∀ a ∈ as, a < 64 := by
-  unfold instMembershipByteArray
+    (xs : Array Swap)
+    (h : as = xs.unzip.fst)
+    (h : as.all (· < size))
+    : ∀ a ∈ as, a < size := by
   grind
 
 theorem idk2
-    (xs : Array (UInt8 × UInt8))
-    (h : bs = ByteArray.mk xs.unzip.snd)
-    (h : bs.data.all (· < 64))
-    : ∀ b ∈ bs, b < 64 := by
-  unfold instMembershipByteArray
+    (xs : Array Swap)
+    (h : bs = xs.unzip.snd)
+    (h : bs.all (· < size))
+    : ∀ b ∈ bs, b < size := by
   grind
 
-def Network.compile (n : Network size) : CompiledNetwork :=
+def Network.compile (n : Network size) : CompiledNetwork size :=
   let swaps := n.toSwaps |>.unzip
   if h : swaps.fst.size = swaps.snd.size ∧ swaps.fst.size < USize.size then
-    let as := ByteArray.mk swaps.fst
-    let bs := ByteArray.mk swaps.snd
-    if h : as.data.all (· < 64) ∧ bs.data.all (· < 64) then
-      have h_as : ∀ a ∈ as, a < 64 := by exact idk1 n.toSwaps rfl h.left
-      have h_bs : ∀ b ∈ bs, b < 64 := by exact idk2 n.toSwaps rfl h.right
+    let as := swaps.fst
+    let bs := swaps.snd
+    if h : as.all (· < size) ∧ bs.all (· < size) then
+      have h_as : ∀ a ∈ as, a < size := idk1 n.toSwaps rfl h.left
+      have h_bs : ∀ b ∈ bs, b < size := idk2 n.toSwaps rfl h.right
       CompiledNetwork.mk as bs (by grind) (by grind) h_as h_bs
     else panic! "invariant #1"
   else panic! "invariant #2"
 
-@[inline]
-partial def CompiledNetwork.run (n : CompiledNetwork) (input : UInt64) : UInt64 :=
-  let rec loop (i : USize) (input : UInt64) : UInt64 :=
+@[grind]
+structure CompiledNetwork.runParallel.h (n : CompiledNetwork size) (vals : Array UInt64) where
+  size_vals_lt : vals.size < USize.size := by grind
+  lt_usize_as : ∀ a ∈ n.as, a < vals.usize := by grind
+  lt_usize_bs : ∀ b ∈ n.bs, b < vals.usize := by grind
+
+partial def CompiledNetwork.runParallel
+    (n : CompiledNetwork size)
+    (vals : Subtype (runParallel.h n ·))
+    : Array UInt64 :=
+  let rec loop
+      (i : USize)
+      (vals : Subtype (runParallel.h n ·))
+      : Array UInt64 :=
     if h : i < n.as.usize then
-      have i_lt_as_size : i.toNat < n.as.size := by grind
-      have i_lt_bs_size : i.toNat < n.bs.size := by grind
+      have i_lt_as_size : i.toNat < n.as.size := by
+        refine (USize.lt_ofNat_iff ?_).mp h <;> grind
+      have i_lt_bs_size : i.toNat < n.bs.size := by
+        refine (USize.lt_ofNat_iff ?_).mp ?_ <;> grind
       let a := n.as.uget i i_lt_as_size
       let b := n.bs.uget i i_lt_bs_size
-      have a_lt : a < 64 := by
-        have : a ∈ n.as := Array.mem_of_getElem rfl
-        exact n.as_all_lt_64 a this
-      have b_lt : b < 64 := by
-        have : b ∈ n.bs := Array.mem_of_getElem rfl
-        exact n.bs_all_lt_64 b this
-      loop (i + 1) (binaryCompareAndSwap ⟨b, b_lt⟩ ⟨a, a_lt⟩ input)
-    else input
-  loop 0 input
+      have : a ∈ n.as := Array.mem_of_getElem rfl
+      have : b ∈ n.bs := Array.mem_of_getElem rfl
+      have vals_property := vals.property
+      let vals := ⟨vals, by grind⟩
+      let vals' := binaryParallelCompareAndSwap a b vals
+      have size_eq := binaryParallelCompareAndSwap_size_eq a b vals
+      have runParallel_h : runParallel.h n vals' := by
+        apply runParallel.h.mk
+        all_goals simp only [size_eq, vals']
+        . exact vals_property.size_vals_lt
+        all_goals simp only [Array.usize, size_eq, Nat.toUSize_eq]
+        . exact vals_property.lt_usize_as
+        . exact vals_property.lt_usize_bs
+      loop (i + 1) ⟨vals', by grind⟩
+    else vals
+  loop 0 vals
 
-@[inline]
-def UInt64.bitsSorted (n : UInt64) : Bool :=
-  let n := n ^^^ (n >>> 1)
-  n &&& (n - 1) = 0
+/--
+Packs the bits of each element of `src` into `dest` like so:
+```
+src  [0b0000,
+      0b0001,
+      0b0010,
+      0b0011,
+      0b0100,
+      0b0101,
+      0b0110,
+      0b0111, ------------------------\
+      0b1000,                          \
+      0b1001,                           \
+      0b1010,                            \
+      0b1011,                            |
+      0b1100,                            |
+      0b1101,                            |
+      0b1110,                            |
+      0b1111]                            v
 
-@[inline]
-def CompiledNetwork.correctlySortsInput (n : CompiledNetwork) (input : UInt64) : Bool :=
-  n.run input |>.bitsSorted
-
-def Network.output (n : Network size) : Std.HashSet UInt64 := Id.run do
-  let mut result := default
-  let numInputs := 2 ^ size.toNat
-  let n := n.compile
-  for i in [0:numInputs] do
-    let output := n.run i.toUInt64
-    result := result.insert output
-  result
-
-partial def Network.correctnessScore (n : Network size) : Nat × Nat :=
-  let size : UInt64 := size.toUInt64
-  let n := n.compile
+dest [0b0000000000000000000000000000000000000000000000001010101010101010,
+      0b0000000000000000000000000000000000000000000000001100110011001100,
+      0b0000000000000000000000000000000000000000000000001111000011110000,
+      0b0000000000000000000000000000000000000000000000001111111100000000]
+```
+-/
+partial def pack
+    -- (size : USize)
+    (src dest : Array UInt64)
+    -- (size_src : src.usize = 64)
+    -- (size_dest : dest.usize = size)
+    : Array UInt64 /- result.size = size -/ :=
   let rec loop
-      (i : UInt64)
-      (successes : Nat)
-      (failures : Nat)
-      : Nat × Nat :=
-    let (successes, failures) :=
-      if n.correctlySortsInput i then
-        (successes + 1, failures)
-      else
-        (successes, failures + 1)
-    let i := LFSR.rand64 size i
-    if i = 1 then
-      (successes, failures)
-    else
-      loop i successes failures
-  loop 1 0 0
+      (dest : Array UInt64)
+      (bitIdx : USize)
+      : Array UInt64 :=
+    if bitIdx < 64 then
+      let rec loop2
+          (dest : Array UInt64)
+          (testCaseIdx : USize)
+          : Array UInt64 :=
+        if testCaseIdx < src.usize ∧ testCaseIdx < dest.usize then
+          let bitIdx64 := bitIdx.toUInt64
+          let bit := 1 &&& src[bitIdx]! >>> testCaseIdx.toUInt64
+          let dest := dest.set! testCaseIdx.toNat <|
+            (dest[testCaseIdx]! &&& ~~~(1 <<< bitIdx64))
+            ||| (bit <<< bitIdx64)
+          loop2 dest (testCaseIdx + 1)
+        else dest
+      let dest := loop2 dest 0
+      loop dest (bitIdx + 1)
+    else dest
+  loop dest 0
 
-def Network.correctnessScore' (n : Network size) : Nat × Nat := Id.run do
-  let mut successes := 0
-  let mut failures := 0
-  let mut start : UInt64 := 1
-  let mut i := start
-  let n := n.compile
-  while true do
-    if n.correctlySortsInput i then
-      successes := successes + 1
-    else
-      failures := failures + 1
-    i := LFSR.rand64 size.toUInt64 i
-    if i = 1 then
+-- theorem pack_size_eq : (pack src dest).size = dest.size := by
+--   unfold pack
+
+
+def mkParallelInputChunk
+    (size : USize)
+    (src dest : Array UInt64)
+    -- (size_src : src.usize = 64)
+    -- (size_dest : dest.usize = size)
+    (seed : UInt64)
+    : Array UInt64 × UInt64 /- result.fst.usize = size, result.snd is the new seed -/
+    := Id.run do
+  let mut src := src
+  let mut seed := seed
+  for testCase in [0:64] do
+    let nextSeed := LFSR.rand64 size.toUInt64 seed
+    src := src.set! testCase seed
+    seed := nextSeed
+    if seed = 1 then
       break
-  (successes, failures)
+  let dest := pack src dest
+  (dest, seed)
+
+-- def pic1xSeed := mkParallelInputChunk 4 (Array.replicate 64 0) (Array.replicate 4 0) 1
+-- def pic1 := pic1xSeed.fst
+-- def myNw := CompiledNetwork.mk (size := 4) #[0, 1, 0, 2, 1] #[2, 3, 1, 3, 2] sorry sorry sorry sorry
+-- def pic1Output := myNw.runParallel ⟨pic1, sorry⟩
+-- #eval! IO.println <| pic1 |>.map (·.toBitString)
+-- #eval! IO.println <| pic1Output |>.map (·.toBitString)
+
+-- def UInt64.MAX : UInt64 := ~~~0
+
+/-- Returns the number of `1`s in the binary representation of `u`. -/
+def UInt64.countSetBits (u : UInt64) : UInt64 := Id.run do
+  let mut u := u
+  for h : i in [0:6] do
+    u := ((u &&& masksA[i]) >>> 2^i) + (u &&& masksB[i])
+  u
+where
+  masksA : Vector UInt64 6 := #[
+    0b1010101010101010101010101010101010101010101010101010101010101010,
+    0b1100110011001100110011001100110011001100110011001100110011001100,
+    0b1111000011110000111100001111000011110000111100001111000011110000,
+    0b1111111100000000111111110000000011111111000000001111111100000000,
+    0b1111111111111111000000000000000011111111111111110000000000000000,
+    0b1111111111111111111111111111111100000000000000000000000000000000,
+  ].toVector
+  masksB : Vector UInt64 6 := #[
+    0b0101010101010101010101010101010101010101010101010101010101010101,
+    0b0011001100110011001100110011001100110011001100110011001100110011,
+    0b0000111100001111000011110000111100001111000011110000111100001111,
+    0b0000000011111111000000001111111100000000111111110000000011111111,
+    0b0000000000000000111111111111111100000000000000001111111111111111,
+    0b0000000000000000000000000000000011111111111111111111111111111111,
+  ].toVector
+
+partial def ParallelChunk.countNotSorted (chunk : Array UInt64) : UInt64 :=
+  let rec loop (i : USize) (acc : UInt64) : UInt64 :=
+    if i + 1 < chunk.usize then
+      let acc := acc ||| chunk[i]! &&& ~~~chunk[i + 1]!
+      loop (i + 1) acc
+    else acc
+  loop 0 0 |>.countSetBits
+
+theorem size_eq_of_size_lt_size_USize_of_usize_eq
+    (dest : Array α)
+    (h : dest.usize = size)
+    (h2 : dest.size < USize.size)
+    : dest.size = size.toNat := by
+  rw [← h]
+  exact Eq.symm (USize.toNat_ofNat_of_lt' h2)
+
+def CompiledNetwork.countTestFailures (c : CompiledNetwork size) : UInt64 := Id.run do
+  let mut seed := 1
+  let mut src := Array.replicate 64 0
+  let mut dest := Array.replicate size.toNat 0
+  let mut failures := 0
+  let mut isFirstIteration := true
+  while seed ≠ 1 ∨ isFirstIteration do
+    isFirstIteration := false
+    (dest, seed) := mkParallelInputChunk size src dest seed
+    if h : dest.usize = size ∧ dest.size < USize.size then
+      -- This `if` is a lazy hack to avoid proving properties of the program.
+      -- Eventually it should be surplanted by compile-time proofs.
+      have runParallel_h : runParallel.h c dest := by
+        refine { size_vals_lt := ?_, lt_usize_as := ?_, lt_usize_bs := ?_ }
+        . rw [size_eq_of_size_lt_size_USize_of_usize_eq dest h.left h.right]
+          exact USize.toNat_lt_two_pow_numBits size
+        . rw [h.left]
+          intro a mem_a
+          exact c.as_sizes a mem_a
+        . grind
+      dest := c.runParallel ⟨dest, runParallel_h⟩
+      failures := failures + ParallelChunk.countNotSorted dest
+    else panic! "invariants violated"
+  failures
+
+-- def myNw := CompiledNetwork.mk (size := 4) #[0, 1, 0, 2, 1] #[2, 3, 1, 3, 2] sorry sorry sorry sorry
+-- #eval! myNw.countTestFailures
+
+-- #eval ParallelChunk.countNotSorted #[0b001000000001000,
+--                                      0b011110010000010,
+--                                      0b111111111110000,
+--                                      0b111111111111111]
+
+/-
+#[111010110010001,
+  111101011001000,
+  011110101100100,
+  001111010110010]
+#[001000000000000,
+  011110010000000,
+  111111111110000,
+  111111111111111]
+-/
+--
+
+-- def pic1Sorted :=
+
+-- @[inline]
+-- def UInt64.bitsSorted (n : UInt64) : Bool :=
+--   let n := n ^^^ (n >>> 1)
+--   n &&& (n - 1) = 0
+
+-- @[inline]
+-- def CompiledNetwork.correctlySortsInput (n : CompiledNetwork) (input : UInt64) : Bool :=
+--   n.run input |>.bitsSorted
+
+-- def Network.output (n : Network size) : Std.HashSet UInt64 := Id.run do
+--   let mut result := default
+--   let numInputs := 2 ^ size.toNat
+--   let n := n.compile
+--   for i in [0:numInputs] do
+--     let output := n.run i.toUInt64
+--     result := result.insert output
+--   result
+
+-- partial def Network.correctnessScore (n : Network size) : Nat × Nat :=
+--   let size : UInt64 := size.toUInt64
+--   let n := n.compile
+--   let rec loop
+--       (i : UInt64)
+--       (successes : Nat)
+--       (failures : Nat)
+--       : Nat × Nat :=
+--     let (successes, failures) :=
+--       if n.correctlySortsInput i then
+--         (successes + 1, failures)
+--       else
+--         (successes, failures + 1)
+--     let i := LFSR.rand64 size i
+--     if i = 1 then
+--       (successes, failures)
+--     else
+--       loop i successes failures
+--   loop 1 0 0
+
+-- def Network.correctnessScore' (n : Network size) : Nat × Nat := Id.run do
+--   let mut successes := 0
+--   let mut failures := 0
+--   let mut start : UInt64 := 1
+--   let mut i := start
+--   let n := n.compile
+--   while true do
+--     if n.correctlySortsInput i then
+--       successes := successes + 1
+--     else
+--       failures := failures + 1
+--     i := LFSR.rand64 size.toUInt64 i
+--     if i = 1 then
+--       break
+--   (successes, failures)
 
 def Network.swapsScore (n : Network size) : Nat :=
   if size ≤ 1 then
@@ -258,7 +491,7 @@ def Network.layersScore (n : Network size) : Nat :=
     n.toArray.size
 
 def Network.addLayer (n : Network size) : Network size :=
-  Network.mk <| n.toArray.push <| .range size
+  Network.mk <| n.toArray.push <| Array.range size.toNat |>.map (·.toUSize)
 
 def Array.swapRemove! [Inhabited α] (arr : Array α) (i : Nat) (a : α) : Array α × α :=
   let result := arr[i]!
@@ -276,7 +509,7 @@ def ByteArray.swapIfInBounds (ba : ByteArray) (a : UInt8) (b : UInt8) (h : ba.si
 def Network.addSwap
     (n : Network size)
     (layerIdx : Nat)
-    (swap : UInt8 × UInt8)
+    (swap : USize × USize)
     (symmetric : Bool)
     : Network size :=
   let n := if layerIdx = n.toArray.size then n.addLayer else n
@@ -284,11 +517,7 @@ def Network.addSwap
   let b := n.toArray[layerIdx]![swap.snd.toNat]!
   if a = swap.fst ∧ b = swap.snd then
     let (n, layer) := n.toArray.swapRemove! layerIdx .empty
-    let layer :=
-      if h : layer.size < USize.size then
-        layer.swapIfInBounds swap.fst swap.snd h
-      else
-        layer
+    let layer := layer.swapIfInBounds swap.fst.toNat swap.snd.toNat
     let n := Network.mk <| n.set! layerIdx layer
     if symmetric then
       n.addSwap layerIdx (size - 1 - swap.fst, size - 1 - swap.snd) false
@@ -306,34 +535,26 @@ def Network.removeSwap
   if 0 < swaps.size then
     let (a, b) := swaps[swapIdx % swaps.size]!
     let (n, layer) := n.toArray.swapRemove! layerIdx .empty
-    let layer :=
-      if h : layer.size < USize.size then
-        layer.swapIfInBounds a b h
-      else
-        layer
+    let layer := layer.swapIfInBounds a.toNat b.toNat
     let n := Network.mk <| n.set! layerIdx layer
     if symmetric then
       let (n, layer) := n.toArray.swapRemove! layerIdx .empty
-      let layer :=
-        if h : layer.size < USize.size then
-          layer.swapIfInBounds (size - 1 - a) (size - 1 - b) h
-        else
-          layer
+      let layer := layer.swapIfInBounds (size - 1 - a).toNat (size - 1 - b).toNat
       let n := Network.mk <| n.set! layerIdx layer
       n
     else n
   else n
 
-def isUselessLayer (layer : ByteArray) : Bool := Id.run do
+def isUselessLayer (layer : Layer) : Bool := Id.run do
   for i in [0 : layer.size], v in layer.toList do
     if i ≠ v.toNat then
       return false
   true
 
-def Network.removeLayerIfUseless (n : Network size) (layer : Nat) : Network size :=
-  let l := n.toArray[layer]!
+def Network.removeLayerIfUseless (n : Network size) (layerIdx : Nat) : Network size :=
+  let l := n.toArray[layerIdx]!
   if isUselessLayer l then
-    let n := n.toArray.eraseIdx! layer
+    let n := n.toArray.eraseIdx! layerIdx
     Network.mk n
   else
     n
@@ -396,7 +617,7 @@ def Network.addRandomSwap [RandomGen Gen] (n : Network size) (g : Gen) (symmetri
           (fst - 1, fst)
       else
         (fst, snd)
-    let n := n.addSwap layer (fst.toUInt8, snd.toUInt8) symmetric
+    let n := n.addSwap layer (fst.toUSize, snd.toUSize) symmetric
     let n := n.removeRedundancy
     (n, g)
 
@@ -435,16 +656,16 @@ def Network.removeRandomLayer [RandomGen Gen] (n : Network size) (g : Gen) : Net
     let n := Network.mk <| n.toArray.eraseIdx! layer
     (n, g)
 
-def Layer.rotate (arr : ByteArray) (amount : Nat) : ByteArray :=
+def Layer.rotate (arr : Layer) (amount : Nat) : Layer :=
   if arr.size = 0 then
     arr
   else
-    let adjust : UInt8 → UInt8 :=
-      fun n => (n.toNat + amount) % arr.size |>.toUInt8
+    let adjust : USize → USize :=
+      fun n => (n.toNat + amount) % arr.size |>.toUSize
     arr
       |> Layer.toSwaps
       |>.map (fun (a, b) => (adjust a, adjust b))
-      |> Swaps.toLayer arr.size.toUInt8
+      |> Swaps.toLayer arr.usize
 
 def Network.rotateRandomLayer [RandomGen Gen] (n : Network size) (g : Gen) : Network size × Gen :=
   if n.toArray.size < 1 then
@@ -549,10 +770,10 @@ def Network.improve
     (n : Network size)
     (g : Gen)
     (fuel : Nat)
-    (lastFailures : Option Nat)
+    (lastFailures : Option UInt64)
     (symmetric : Bool)
     (numMutations : Nat := (size.toNat * (size.toNat - 1) / 2))
-    : Network size × Gen × Option Nat :=
+    : Network size × Gen × Option UInt64 :=
   if fuel = 0 ∨ size = 0 then
     (n, g, lastFailures)
   else
@@ -564,17 +785,17 @@ def Network.improve
       ∧ (n'.swapsScore ≠ n.swapsScore ∨ n'.layersScore ≠ n.layersScore)
     let (n, g, lastFailures) :=
       if n'IsSmaller then
-        let (_successes, failures) := n'.correctnessScore
+        let failures := n'.compile.countTestFailures
         let n'IsCorrect := failures = 0
         if n'IsCorrect then
-          (n', g, failures)
+          (n', g, some failures)
         else
           (n, g, lastFailures)
       else
         if nIsCorrect then
           (n, g, lastFailures)
         else
-          let (_successes, failures) := n'.correctnessScore
+          let failures := n'.compile.countTestFailures
           (n', g, failures)
     n.improve g (fuel - 1) lastFailures symmetric numMutations
 
@@ -592,18 +813,18 @@ def Network.bubble : Network size :=
 where
   numAscending := (2 * (size - 2) + 1) / 2 + 1
   ascending := .ofFn (n := numAscending.toNat) fun i => Id.run do
-    let mut arr := ByteArray.range size
+    let mut arr := Array.range size.toNat |>.map (·.toUSize)
     let i := i.toNat
     let numSwaps := i / 2 + 1
     for j in [0 : numSwaps] do
       let a := j * 2 + if i % 2 = 0 then 0 else 1
       arr :=
-        if h : arr.size < USize.size then
-          arr.swapIfInBounds a.toUInt8 (a.toUInt8 + 1) h
+        if arr.size < USize.size then
+          arr.swapIfInBounds a (a + 1)
         else arr
     arr
 
-def Network.fromLayerSwapsList (layers : List (List (UInt8 × UInt8))) : Network size :=
+def Network.fromLayerSwapsList (layers : List (List Swap)) : Network size :=
   let layers := layers.map (·.toArray) |>.toArray
   .fromLayerSwaps layers
 
@@ -622,7 +843,7 @@ def nw14_51x10 : Network 14 := .fromLayerSwapsList [[(0,1),(2,3),(4,5),(6,7),(8,
 def nw14_52x9 : Network 14 := .fromLayerSwapsList [[(0,1),(2,3),(4,5),(6,7),(8,9),(10,11),(12,13)],[(0,2),(1,3),(4,8),(5,9),(10,12),(11,13)],[(0,10),(1,6),(2,11),(3,13),(5,8),(7,12)],[(1,4),(2,8),(3,6),(5,11),(7,10),(9,12)],[(0,1),(3,9),(4,10),(5,7),(6,8),(12,13)],[(1,5),(2,4),(3,7),(6,10),(8,12),(9,11)],[(1,2),(3,5),(4,6),(7,9),(8,10),(11,12)],[(2,3),(4,5),(6,7),(8,9),(10,11)],[(3,4),(5,6),(7,8),(9,10)]]
 def nw15_56x10 : Network 15 := .fromLayerSwapsList [[(1,2),(3,10),(4,14),(5,8),(6,13),(7,12),(9,11)],[(0,14),(1,5),(2,8),(3,7),(6,9),(10,12),(11,13)],[(0,7),(1,6),(2,9),(4,10),(5,11),(8,13),(12,14)],[(0,6),(2,4),(3,5),(7,11),(8,10),(9,12),(13,14)],[(0,3),(1,2),(4,7),(5,9),(6,8),(10,11),(12,13)],[(0,1),(2,3),(4,6),(7,9),(10,12),(11,13)],[(1,2),(3,5),(8,10),(11,12)],[(3,4),(5,6),(7,8),(9,10)],[(2,3),(4,5),(6,7),(8,9),(10,11)],[(5,6),(7,8)]]
 
-def goodNetworks : Array (Σ size : UInt8, Network size) :=
+def goodNetworks : Array (Σ size : USize, Network size) :=
   #[
     ⟨6, nw6_12x5⟩,
     ⟨7, nw7_16x6⟩,
